coq-osiris/theories/semantics/eval.v
@@ -1295,6 +1295,8 @@ Fixpoint pre_eval η e {struct e} : microvx :=
   | EFork e1 e2 =>
       '(f, v) ← pair_op Strat.fun_app_order (eval η e1) (eval η e2) ;
       fork f v
+  | ESelf =>
+      self
   | EJoin e =>
       t ← as_thread (eval η e) ;
       join t
